Finished Lemma 4.

proof.v
@@ -4,6 +4,7 @@ Require Import Coq.Init.Datatypes.
 Require Import Coq.Lists.List.
 Require Import Arith.EqNat.
 Require Import Maps.
+Require Import Program.Equality.
 
 Fixpoint list_rel { A : Type } (rel : A -> A -> Prop) (l l' : list A) : Prop :=
   match l, l' with
@@ -27,6 +28,10 @@ Inductive expr : Type :=
 | E_Invk : expr -> method_id -> list expr -> expr
 | E_New : class_id -> list expr -> expr
 | E_Cast : class_id -> expr -> expr.
+
+Inductive exprl : Type :=
+| EL_Expr : expr -> exprl
+| EL_Lib : exprl.
 
 Theorem expr_ind_list :
   forall P : expr -> Prop,
@@ -56,21 +61,17 @@ Inductive class : Type :=
 
 Definition class_table : Type := partial_map class * partial_map class.
 
-
+Definition empty_map {A : Type} : partial_map A := fun _ => None.
+Definition ct_app (ct : class_table) : class_table :=
+  match ct with (app, _) => (app, empty_map) end.
+Definition ct_lib (ct : class_table) : class_table :=
+  match ct with (_, lib) => (empty_map, lib) end.
 Definition lookup (ct : class_table) (i : class_id) : option class :=
   match ct with (app, lib) =>
                 match app i with
                 | Some c => Some c
                 | None => lib i
                 end
-  end.
-Definition lookup_field (c : class) (f : field_id) : option class_id :=
-  match c with
-  | Obj => None
-  | C _ _ fs _ _ => match find (fun fp => beq_id (snd fp) f) fs with
-                   | None => None
-                   | Some (ci, _) => Some ci
-                   end
   end.
 Definition lookup_method (c : class) (mi : method_id) : option method :=
   match c with
@@ -113,6 +114,12 @@ Proof. intros. unfold in_table. left. apply H. Qed.
 Lemma in_lib_in_table : forall (ct : class_table) (c : class),
     in_lib ct c -> in_table ct c.
 Proof. intros. unfold in_table. right. apply H. Qed.
+Lemma in_app_in_table_id : forall (ct : class_table) (ci : class_id),
+    in_app_id ct ci -> in_table_id ct ci.
+Proof. intros. unfold in_table_id. left. apply H. Qed.
+Lemma in_lib_in_table_id : forall (ct : class_table) (ci : class_id),
+    in_lib_id ct ci -> in_table_id ct ci.
+Proof. intros. unfold in_table_id. right. apply H. Qed.
 
 Definition extends (ct : class_table) (c d : class) : Prop :=
   match c with
@@ -127,7 +134,7 @@ Definition extends_id (ct : class_table) (ci di : class_id) : Prop :=
   | Some (C _ di' _ _ _) => di = di'
   end.
 
-Inductive subtype (ct : class_table) : class -> class -> Prop :=
+Inductive subtype (ct : class_table) : class -> class -> Type :=
 | S_Ref : forall (c : class), subtype ct c c
 | S_Trans : forall (c d e : class), subtype ct c d -> subtype ct d e -> subtype ct c e
 | S_Sub : forall (c d : class), extends ct c d -> subtype ct c d.
@@ -136,6 +143,7 @@ Inductive subtype_id (ct : class_table) : class_id -> class_id -> Prop :=
 | SI_Ref : forall ci, in_table_id ct ci -> subtype_id ct ci ci
 | SI_Sub : forall ci di, extends_id ct ci di -> subtype_id ct ci di
 | SI_Trans : forall ci di ei, subtype_id ct ci di -> subtype_id ct di ei -> subtype_id ct ci ei.
+
 
 Inductive valid_class (ct : class_table) : class -> Type :=
 | ValidObj : in_lib ct Obj -> ~ in_app ct Obj -> lookup ct obj_id = Some Obj -> valid_class ct Obj
@@ -150,24 +158,26 @@ Fixpoint mtype (ct : class_table) (mi : method_id) (c : class) (pfc : valid_clas
   option (list class_id * class_id) :=
   match pfc with
   | ValidObj _ _ _ _ => None
-  | ValidParent _ d pfd _ _ _ _ _ =>
+  | ValidParent _ _ d pfd _ _ _ _  =>
     match lookup_method c mi with
-    | None => None
+    | None => mtype ct mi d pfd
     | Some (Method ci _ l_arg _) => Some (map fst l_arg, ci) 
     end
   end.
 
 Fixpoint fields (ct : class_table) (c : class) (pfc : valid_class ct c) : list class_id :=
   match pfc, c with
-  | ValidObj _ _ _ _, _ => nil
   | ValidParent _ _ d pfd _ _ _ _ , C _ _ fs _ _ => map fst fs ++ fields ct d pfd
+  | _, C _ _ fs _ _ => map fst fs
   | _, _ => nil
   end.
 
+Definition lookup_field (ct : class_table) (c : class) (pfc : valid_class ct c) (f : field_id) : option class_id :=
+  find (beq_id f) (fields ct c pfc).
 Inductive type_of (ct : class_table) (gamma : context) : expr -> class_id -> Prop :=
 | T_Var : forall x, type_of ct gamma (E_Var x) (gamma x)
-| T_Field : forall e c di f,
-    type_of ct gamma e (id_of c) -> lookup_field c f = Some di ->
+| T_Field : forall e c pfc di f,
+    type_of ct gamma e (id_of c) -> lookup_field ct c pfc f = Some di ->
     type_of ct gamma (E_Field e f) di
 | T_Invk : forall e0 c0 ci0 pfc0 ld ret mi le lc,
     id_of c0 = ci0 -> type_of ct gamma e0 ci0 -> mtype ct mi c0 pfc0 = Some (ld, ret) ->
@@ -183,30 +193,58 @@ Inductive type_of (ct : class_table) (gamma : context) : expr -> class_id -> Pro
     type_of ct gamma (E_New ci le) ci
 | T_Cast : forall e0 ci di, type_of ct gamma e0 di -> type_of ct gamma (E_Cast ci e0) ci.
 
+Check type_of_ind.
+Theorem type_of_ind_list : forall (ct : class_table) (gamma : context) (P : expr -> class_id -> Prop),
+       (forall x : var, P (E_Var x) (gamma x)) ->
+       (forall (e : expr) (c : class) (pfc : valid_class ct c) (di : class_id) (f0 : field_id),
+        type_of ct gamma e (id_of c) -> P e (id_of c) -> lookup_field ct c pfc f0 = Some di -> P (E_Field e f0) di) ->
+       (forall (e0 : expr) (c0 : class) (ci0 : class_id) (pfc0 : valid_class ct c0) (ld : list class_id)
+          (ret : class_id) (mi : method_id) (le : list expr) (lc : list class_id),
+        id_of c0 = ci0 ->
+        type_of ct gamma e0 ci0 ->
+        P e0 ci0 ->
+        mtype ct mi c0 pfc0 = Some (ld, ret) ->
+        length ld = length le ->
+        length le = length lc ->
+        Forall (fun p : expr * class_id => type_of ct gamma (fst p) (snd p)) (combine le lc) ->
+        Forall (fun p : expr * class_id => P (fst p) (snd p)) (combine le lc) ->
+        Forall (fun p : class_id * class_id => subtype_id ct (fst p) (snd p)) (combine lc ld) ->
+        P (E_Invk e0 mi le) ci0) ->
+       (forall (c : class) (ci : class_id) (pfc : valid_class ct c) (le : list expr) (lc ld : list class_id),
+        id_of c = ci ->
+        fields ct c pfc = ld ->
+        length ld = length le ->
+        length le = length lc ->
+        Forall (fun p : expr * class_id => type_of ct gamma (fst p) (snd p)) (combine le lc) ->
+        Forall (fun p : expr * class_id => P (fst p) (snd p)) (combine le lc) ->
+        Forall (fun p : class_id * class_id => subtype_id ct (fst p) (snd p)) (combine lc ld) -> P (E_New ci le) ci) ->
+       (forall (e0 : expr) (ci di : class_id), type_of ct gamma e0 di -> P e0 di -> P (E_Cast ci e0) ci) ->
+       forall (e : expr) (c : class_id), type_of ct gamma e c -> P e c.
+  admit.
+Admitted.
+
 Inductive type_checks (ct : class_table) (gamma : context) : expr -> Prop :=
 | TC_Var : forall x, in_table_id ct (gamma x) -> type_checks ct gamma (E_Var x)
 | TC_Field : forall e f di, type_of ct gamma (E_Field e f) di -> in_table_id ct di -> type_checks ct gamma e ->
                        type_checks ct gamma (E_Field e f)
+| TC_New : forall ci le, in_table_id ct ci -> Forall (type_checks ct gamma) le -> type_checks ct gamma (E_New ci le)
 | TC_Invk : forall e m le di, type_of ct gamma (E_Invk e m le) di -> in_table_id ct di ->
                       type_checks ct gamma e -> Forall (type_checks ct gamma) le ->
                       type_checks ct gamma (E_Invk e m le)
-| TC_New : forall ci le, in_table_id ct ci -> Forall (type_checks ct gamma) le -> type_checks ct gamma (E_New ci le)
 | TC_Cast : forall e di, in_table_id ct di -> type_checks ct gamma e -> type_checks ct gamma (E_Cast di e).
-(*  exists c, type_of ct gamma e c /\ in_table_id ct c. *)
 
-  
-Definition valid_table (ct : class_table) : Type :=
-  forall c, in_table ct c -> valid_class ct c.
-
-Lemma extends_injective : forall ct c d d',
-    valid_class ct c -> extends ct c d -> extends ct c d' -> d = d'.
-Proof.
-  intros ct c d d' pfc c_ext_d c_ext_d'.
-  unfold extends in c_ext_d, c_ext_d'. destruct c as [| ci di k ms fs].
-  - inversion c_ext_d.
-  - rewrite c_ext_d in c_ext_d'. inversion c_ext_d'. reflexivity.
-Qed.
-
+Definition dfields (c : class) : list field_id :=
+  match c with
+  | Obj => nil
+  | C _ _ fs _ _ => map snd fs
+  end.
+Fixpoint declaring_class (ct : class_table) (c : class) (pfc : valid_class ct c) (f : field_id) : option class_id :=
+  match pfc with
+  | ValidObj _ _ _ _ => None
+  | ValidParent _ _ d pfd _ _ _ _ => if (existsb (fun f' => beq_id f' f) (dfields c))
+                                    then Some (id_of c)
+                                    else declaring_class ct d pfd f
+  end.
 Definition dmethods (c : class) : list method_id :=
   match c with
   | Obj => nil
@@ -220,6 +258,41 @@ Fixpoint mresolve (ct : class_table) (m : method_id) (c : class) (pfc : valid_cl
                                       then Some c
                                       else mresolve ct m d pfd
   end.
+
+Inductive valid_expr (ct : class_table) (gamma : context) : expr -> Prop :=
+| Val_Var : forall x, type_checks ct gamma (E_Var x) -> valid_expr ct gamma (E_Var x)
+| Val_Field : forall e f ci c pfc,
+    type_checks ct gamma (E_Field e f) ->
+    type_of ct gamma e ci -> id_of c = ci ->
+    declaring_class ct c pfc f <> None ->
+    valid_expr ct gamma e ->
+    valid_expr ct gamma (E_Field e f)
+| Val_New : forall ci le,
+    type_checks ct gamma (E_New ci le) ->
+    Forall (valid_expr ct gamma) le ->
+    valid_expr ct gamma (E_New ci le)
+| Val_Invk : forall e m le ci c pfc,
+    type_checks ct gamma (E_Invk e m le) ->
+    valid_expr ct gamma e ->
+    Forall (valid_expr ct gamma) le ->
+    type_of ct gamma e ci -> id_of c = ci ->
+    mresolve ct m c pfc <> None ->
+    valid_expr ct gamma (E_Invk e m le)
+| Val_Cast : forall ci e,
+    type_checks ct gamma (E_Cast ci e) -> valid_expr ct gamma e -> valid_expr ct gamma (E_Cast ci e).
+Inductive valid_table : class_table -> Prop :=
+| VT : forall ct, (forall c, in_table ct c -> valid_class ct c) ->
+             (forall c ci, lookup ct ci = Some c -> id_of c = ci) ->
+             valid_table ct.
+
+Lemma extends_injective : forall ct c d d',
+    valid_class ct c -> extends ct c d -> extends ct c d' -> d = d'.
+Proof.
+  intros ct c d d' pfc c_ext_d c_ext_d'.
+  unfold extends in c_ext_d, c_ext_d'. destruct c as [| ci di k ms fs].
+  - inversion c_ext_d.
+  - rewrite c_ext_d in c_ext_d'. inversion c_ext_d'. reflexivity.
+Qed.
 
 Lemma mres_lib_in_lib : forall (ct : class_table) (m : method_id) (c e : class) (pfc : valid_class ct c),
     in_lib ct c -> mresolve ct m c pfc = Some e -> in_lib ct e.
@@ -246,22 +319,44 @@ Lemma lib'_subset_lib : forall (ct ct' : class_table) (c : class),
     ave_rel ct ct' -> in_table ct' c -> in_lib ct c -> in_lib ct' c.
 Proof.
   intros. inversion H. unfold in_table in H0. destruct H0.
-  - apply H2 in H0. unfold valid_table in X.
+  - apply H4 in H0. destruct H2.
     assert (in_table ct c). { apply in_app_in_table. apply H0. }
-    apply X in H5. inversion H5.
-    + rewrite <- H9 in H0. unfold not in H7. apply H7 in H0. inversion H0.
-    + destruct H8. split. apply H1. apply H0. 
+    apply H2 in H8. inversion H8.
+    + rewrite <- H12 in H0. unfold not in H10. apply H10 in H0. inversion H0.
+    + destruct H11. split. apply H1. apply H0. 
   - apply H0.
 Qed.
 
-Inductive alpha (ct ct' : class_table) (pft : ave_rel ct ct') : expr * expr -> Prop :=
-| Rel_Field : forall e e' f, alpha ct ct' pft (e, e') -> alpha ct ct' pft (E_Field e f, E_Field e' f)
-| Rel_Invk : forall e e' le le' m, alpha ct ct' pft (e, e') -> length le = length le' -> Forall (alpha ct ct' pft) (combine le le') ->
-                              alpha ct ct' pft (E_Invk e m le, E_Invk e' m le')
+Inductive alpha (ct ct' : class_table) (pft : ave_rel ct ct') (gamma : context) : exprl * exprl -> Prop :=
+| Rel_Field : forall e e' f,
+    alpha ct ct' pft gamma (EL_Expr e, EL_Expr e') ->
+    alpha ct ct' pft gamma (EL_Expr (E_Field e f), EL_Expr (E_Field e' f))
+| Rel_Lib_Field : forall e ci c pfc f,
+    alpha ct ct' pft gamma (EL_Expr e, EL_Lib) ->
+    declaring_class ct c pfc f = Some ci -> in_lib_id ct ci ->
+    type_of ct gamma e (id_of c) ->
+    alpha ct ct' pft gamma (EL_Expr (E_Field e f), EL_Lib)
 | Rel_New : forall ci le le', in_table_id ct' ci -> length le = length le' ->
-                         Forall (alpha ct ct' pft) (combine le le') ->
-                         alpha ct ct' pft (E_New ci le, E_New ci le')
-| Rel_Cast : forall e e' c, alpha ct ct' pft (e, e') -> alpha ct ct' pft (E_Cast c e, E_Cast c e').
+                         Forall (alpha ct ct' pft gamma) (combine (map EL_Expr le) (map EL_Expr le')) ->
+                         alpha ct ct' pft gamma (EL_Expr (E_New ci le), EL_Expr (E_New ci le'))
+| Rel_Lib_New : forall ci le,
+    in_lib_id ct ci -> Forall (fun e => alpha ct ct' pft gamma (EL_Expr e, EL_Lib)) le ->
+    alpha ct ct' pft gamma (EL_Expr (E_New ci le), EL_Lib)
+| Rel_Invk : forall e e' le le' m,
+    alpha ct ct' pft gamma (EL_Expr e, EL_Expr e') ->
+    length le = length le' ->
+    Forall (alpha ct ct' pft gamma) (combine (map EL_Expr le) (map EL_Expr le')) ->
+    alpha ct ct' pft gamma (EL_Expr (E_Invk e m le), EL_Expr (E_Invk e' m le'))
+| Rel_Lib_Invk : forall e le mi,
+    (exists c, in_lib ct c /\ In mi (dmethods c)) ->
+    alpha ct ct' pft gamma (EL_Expr e, EL_Lib) ->
+    Forall (fun e' => alpha ct ct' pft gamma (EL_Expr e', EL_Lib)) le ->
+    alpha ct ct' pft gamma (EL_Expr (E_Invk e mi le), EL_Lib)
+| Rel_Cast : forall e e' c, alpha ct ct' pft gamma (EL_Expr e, EL_Expr e') ->
+                       alpha ct ct' pft gamma (EL_Expr (E_Cast c e), EL_Expr (E_Cast c e'))
+| Rel_Lib_Cast : forall e ci,
+    alpha ct ct' pft gamma (EL_Expr e, EL_Lib) -> alpha ct ct' pft gamma (EL_Expr (E_Cast ci e), EL_Lib).
+    
 
 Definition subst := var -> expr.
 
@@ -273,6 +368,373 @@ Fixpoint do_sub (sig : subst) (e : expr) : expr :=
  | E_New c es => E_New c (map (do_sub sig) es)
  | E_Cast c e' => E_Cast c (do_sub sig e')
  end.
+
+Axiom sub_keep_typ : forall (ct : class_table) (sig : subst) (gamma : context) (e : expr) (c : class_id),
+    type_of ct gamma e c -> type_of ct gamma (do_sub sig e) c.
+Lemma eq_valid : forall (ct : class_table) (c d : class) (pfc : valid_class ct c),
+    c = d -> valid_class ct d.
+Proof.
+  intros ct c d pfc cdeq.
+  destruct pfc.
+  - rewrite <- cdeq. apply ValidObj. trivial. trivial. trivial.
+  - apply ValidParent with d0.
+    + trivial.
+    + rewrite <- cdeq. trivial.
+    + rewrite <- cdeq. trivial.
+    + rewrite <- cdeq. trivial.
+    + rewrite <- cdeq. trivial.
+Qed.
+
+Lemma id_eq : forall (ct : class_table) c d (pfc : valid_class ct c) (pfd : valid_class ct d),
+    id_of c = id_of d -> c = d.
+Proof.
+  intros ct c d pfc pfd eq_id.
+  inversion pfc.
+  - inversion pfd.
+    + reflexivity.
+    + rewrite <- H2 in eq_id; unfold id_of at 1 in eq_id; rewrite <- eq_id in H7.
+      rewrite H1 in H7; inversion H7; reflexivity.
+  - inversion pfd.
+    + rewrite <- H8 in eq_id; unfold id_of at 2 in eq_id; rewrite eq_id in H3.
+      rewrite H3 in H7; inversion H7; reflexivity.
+    + rewrite eq_id in H3. rewrite H9 in H3. inversion H3. reflexivity.
+Qed.
+
+Lemma valid_in_table : forall (ct : class_table) (c : class) (pfc : valid_class ct c),
+    in_table ct c.
+Proof.
+  intros ct c pfc. inversion pfc.
+  - apply in_lib_in_table. apply H.
+  - destruct H2.
+    * apply H2.
+    * apply in_app_in_table. apply H2.
+Qed.
+
+Lemma in_ct_lib_in_lib : forall (ct : class_table) (c : class),
+    in_table (ct_lib ct) c -> in_lib ct c.
+Proof.
+  intros ct c in_ct_lib.
+  unfold ct_lib, in_table in in_ct_lib; unfold in_lib; destruct ct.
+  destruct in_ct_lib.
+  - unfold in_app in H. unfold empty_map in H. destruct H. reflexivity.
+  - unfold in_lib in H. apply H.
+Qed.
+
+Lemma valid_table_valid_lib : forall ct,
+    valid_table ct -> valid_table (ct_lib ct).
+Proof.
+  intros. destruct H.
+  apply VT.
+  - intros.
+    assert (valid_class ct c) as pfc.
+    { apply H. apply in_lib_in_table. apply in_ct_lib_in_lib. trivial. }
+    destruct ct as [app lib]. induction pfc.
+    + apply ValidObj.
+      * simpl. simpl in i. trivial.
+      * simpl. unfold empty_map. unfold not. intros. apply H2. trivial.
+      * simpl. simpl in e. simpl in n. destruct (app obj_id); trivial.
+        unfold not in n. assert False. { apply n. intros. inversion H2. } contradiction.
+    + apply ValidParent with d.
+      * apply IHpfc. unfold in_table. simpl. right. inversion pfc; trivial.
+        destruct o as [[don _] | [_ con]]; trivial.
+        destruct n. split; trivial. apply in_ct_lib_in_lib. trivial.
+      * destruct c; trivial.
+        simpl. simpl in e. destruct (app c0) eqn:d_in_app; trivial.
+        inversion e. rewrite H3 in d_in_app. destruct o.
+        -- inversion pfc.
+           ++ simpl in H5.
+              assert (lookup (app, lib) c0 = Some d).
+              { simpl. rewrite d_in_app. reflexivity. }
+              apply H0 in H8. destruct H5. rewrite <- H7 in H8. simpl in H8. rewrite <- H8 in d_in_app.
+              rewrite d_in_app. unfold not. intros. inversion H5.
+           ++ destruct H2. destruct H6. split; trivial.
+              simpl.
+              assert (id_of d = c0).
+              { apply H0. simpl. rewrite d_in_app. reflexivity. }
+              rewrite H6. rewrite d_in_app. unfold not. intros. inversion H11.
+        -- simpl in H1. unfold in_table in H1. destruct H1.
+           ++ unfold empty_map in H1. simpl in H1. destruct H1. trivial.
+           ++ simpl in H1. destruct H2. simpl in H4. destruct n. split; trivial.
+      * simpl. unfold empty_map. unfold not. intros. destruct H2. apply H3. trivial.
+      * left. split; trivial.
+        destruct o; destruct H2; trivial.
+        apply in_ct_lib_in_lib in H1. destruct n. split; trivial.
+      * simpl. simpl in e0. destruct (app (id_of c)) eqn:c_in_app; trivial.
+        apply in_ct_lib_in_lib in H1. destruct n. split; trivial.
+        simpl. unfold not. intros. rewrite H2 in c_in_app. inversion c_in_app.
+  - destruct ct as [app lib].
+    intros. simpl in H1. apply H0. simpl. destruct (app ci) eqn:c_in_app; trivial.
+    assert (id_of c0 = ci).
+    { apply H0. simpl. rewrite c_in_app. reflexivity. }
+    assert (valid_class (app, lib) c0).
+    { apply H. unfold in_table. simpl. left. rewrite H2.
+      unfold not. intro. rewrite c_in_app in H3. inversion H3. }
+    inversion H3.
+    + rewrite <- H7 in H2. simpl in H2. rewrite <- H2 in c_in_app. simpl in H5. destruct H5.
+      unfold not. intro. rewrite H5 in c_in_app. inversion c_in_app.
+    + destruct H6. simpl. split.
+      * rewrite H2. unfold not. intro. rewrite H1 in H6. inversion H6.
+      * rewrite H2. unfold not. intro. rewrite c_in_app in H6. inversion H6.
+Qed.
+
+Lemma in_ct_lib_in_lib_id : forall (ct : class_table) (ci : class_id),
+    in_table_id (ct_lib ct) ci -> in_lib_id ct ci.
+Proof.
+  intros ct c in_ct_lib_id.
+  unfold ct_lib, in_table_id in in_ct_lib_id; unfold in_lib_id; destruct ct.
+  destruct in_ct_lib_id.
+  - unfold in_app_id in H. unfold empty_map in H. destruct H. reflexivity.
+  - unfold in_lib_id in H. apply H.
+Qed.
+
+Lemma valid_obj_Valid_Obj : forall ct (pfc : valid_class ct Obj), exists h1 h2 h3,
+    pfc = ValidObj ct h1 h2 h3.
+Proof.
+  intros ct pfc. dependent destruction pfc.
+  - exists i, n, e. reflexivity.
+  - inversion e.
+Qed.
+
+Lemma lookup_self :
+  forall ct c (pfc : valid_class ct c),
+    lookup ct (id_of c) = Some c.
+Proof. intros. inversion pfc; trivial. Qed.
+
+Lemma ext_in_lib_ext_in_ct :
+  forall (ct : class_table) (pft : valid_table ct) (c d : class) (pfd : valid_class ct d),
+    extends (ct_lib ct) c d -> extends ct c d.
+Proof.
+  intros ct pft c d pfd ext_in_lib.
+  destruct c.
+  - inversion ext_in_lib.
+  - simpl. simpl in ext_in_lib.
+    assert (id_of d = c0).
+    { apply valid_table_valid_lib in pft. inversion pft. apply H0. trivial. }
+    rewrite <- H. apply lookup_self. trivial.
+Qed.
+
+Lemma ext_in_lib_ext_in_ct_id :
+  forall (ct : class_table) (pft : valid_table ct) (ci di : class_id),
+    in_table_id ct ci -> extends_id (ct_lib ct) ci di -> extends_id ct ci di.
+Proof.
+  intros ct pft ci di ci_in_ct ext_in_lib.
+  
+Admitted.
+
+Lemma valid_in_lib_in_lib : forall ct c (pfc : valid_class (ct_lib ct) c),
+    in_lib ct c.
+Proof.
+  intros ct c pfc.
+  destruct ct as [app lib]. simpl.
+  apply valid_in_table in pfc. unfold in_table in pfc. destruct pfc.
+  - simpl in H. unfold empty_map in H. destruct H. trivial.
+  - simpl in H. trivial.
+Qed.
+
+Lemma decl_in_lib_in_lib : forall ct c (pfc : valid_class (ct_lib ct) c) f di,
+    declaring_class (ct_lib ct) c pfc f = Some di -> in_lib_id ct di.
+Proof.
+  intros ct c pfc f di decl_in_lib.
+  remember pfc as pfc'.
+  induction pfc'.
+  - simpl in decl_in_lib. inversion decl_in_lib.
+  - simpl in decl_in_lib. destruct (existsb (fun f' : id => beq_id f' f) (dfields c)).
+    + inversion decl_in_lib. destruct ct as [app lib]. simpl. clear Heqpfc'.
+      apply valid_in_lib_in_lib in pfc. simpl in pfc. trivial.
+    + apply IHpfc' with pfc'. trivial. trivial.
+Qed.
+
+Lemma supertype_valid : forall (ct : class_table) (c d : class) (pfc : valid_class ct c),
+    subtype ct c d -> valid_class ct d.
+Proof.
+  intros ct c d pfc subtyp. induction subtyp.
+  - eauto. 
+  - eauto. 
+  - inversion pfc.
+    + rewrite <- H2 in e. unfold extends in e. inversion e.
+    + assert (d = d0).
+      { apply extends_injective with (c := c) (ct := ct). eauto. eauto. eauto. }
+      rewrite H5; eauto.
+Qed.
+
+Lemma supertype_lib_in_lib : forall (ct : class_table) (c d : class) (pfc : valid_class ct c), 
+    subtype ct c d -> in_lib ct c -> in_lib ct d.
+Proof.
+  intros ct c d pfc subtyp c_in_lib. induction subtyp.
+  - apply c_in_lib.
+  - apply IHsubtyp2.
+    apply supertype_valid with (c := c). eauto. eauto.
+    apply IHsubtyp1. eauto. eauto.
+  - inversion pfc.
+    + rewrite <- H2 in e. unfold extends in e. inversion e.
+    + assert (d = d0).
+      { apply extends_injective with (c:= c) (ct := ct). eauto. eauto. eauto. }
+      destruct H2.
+      * destruct H2. rewrite H5. eauto.
+      * destruct H2. destruct H1. split. apply c_in_lib. apply H6.
+Qed.
+
+Lemma lib_par_same : forall ct (pft : valid_table ct) c d pfc_l pfd_l ext nla sca lk pfc,
+    pfc_l = ValidParent (ct_lib ct) c d pfd_l ext nla sca lk ->
+    exists ext' nla' sca' lk' pfd, pfc = ValidParent ct c d pfd ext' nla' sca' lk'.
+Proof.
+  intros. remember pfc as pfc'. destruct pfc.
+  - inversion ext.
+  - assert (d = d0) as deq.
+    { apply extends_injective with ct c; trivial.
+      - inversion pft. apply ext_in_lib_ext_in_ct; trivial.
+         apply H0. apply in_lib_in_table. apply valid_in_lib_in_lib. trivial. }
+    rewrite deq.
+    exists e, n, o, e0, pfc. trivial.
+Qed.
+
+Lemma simul_induct_lib :
+  forall (ct : class_table) (pft : valid_table ct) (P : forall ct c, valid_class (ct_lib ct) c -> valid_class ct c -> Prop),
+    (forall o1 o2 o3 o1' o2' o3', P ct Obj (ValidObj (ct_lib ct) o1 o2 o3) (ValidObj ct o1' o2' o3')) ->
+    (forall c d pfd_l pfd ext nla sca lk ext' nla' sca' lk',
+        P ct d pfd_l pfd ->
+        P ct c (ValidParent (ct_lib ct) c d pfd_l ext nla sca lk) (ValidParent ct c d pfd ext' nla' sca' lk')) ->
+    forall c pfc_l pfc, P ct c pfc_l pfc.
+Proof. 
+  intros ct pft P Hobj Hind c pfc_l. 
+  remember pfc_l as pfc_lr. induction pfc_l.
+  - intros. assert (exists h1 h2 h3, pfc = ValidObj ct h1 h2 h3). apply valid_obj_Valid_Obj.
+    destruct H as [x [y [z id]]]. rewrite id. rewrite Heqpfc_lr. apply Hobj.
+  - intros. assert (exists ext' nla' sca' lk' pfd, pfc = ValidParent ct c d pfd ext' nla' sca' lk').
+    { apply lib_par_same with pfc_lr pfc_l e n o e0; trivial. }
+    destruct H as [ext' [nla' [sca' [lk' [pfd H']]]]].
+    rewrite H'. rewrite Heqpfc_lr. apply Hind. apply IHpfc_l. trivial.
+Qed.
+Lemma rel_par_same : forall ct ct' (rel : ave_rel ct ct') c d pfc pfd ext nla sca lk pfc',
+    pfc = ValidParent ct c d pfd ext nla sca lk ->
+    exists ext' nla' sca' lk' pfd', pfc' = ValidParent ct' c d pfd' ext' nla' sca' lk'.
+Proof.
+  intros. remember pfc' as pfc''. inversion rel as [val_ct val_ct' keep_app keep_ext keep_lib]. destruct pfc'.
+  - inversion ext.
+  - assert (d = d0) as deq.
+    { apply extends_injective with ct' c.
+      - trivial.
+      - apply keep_ext.
+        + trivial.
+        + destruct o.
+          * apply a.
+          * apply in_app_in_table. apply a.
+      - trivial. }
+    rewrite deq.
+    exists e, n, o, e0, pfc'. trivial.
+Qed.
+
+Lemma simul_induct :
+  forall (ct ct' : class_table) (rel : ave_rel ct ct') 
+    (P : forall ct ct' rel c, valid_class ct c -> valid_class ct' c -> Prop),
+    (forall o1 o2 o3 o1' o2' o3', P ct ct' rel Obj (ValidObj ct o1 o2 o3) (ValidObj ct' o1' o2' o3')) ->
+    (forall c d pfd pfd' ext nla sca lk ext' nla' sca' lk', P ct ct' rel d pfd pfd' ->
+        P ct ct' rel c (ValidParent ct c d pfd ext nla sca lk) (ValidParent ct' c d pfd' ext' nla' sca' lk')) ->
+    forall c pfc pfc', P ct ct' rel c pfc pfc'.
+Proof. 
+  intros ct ct' rel P Hobj Hind c pfc. inversion rel as [val_ct val_ct' keep_app keep_ext keep_lib].
+  remember pfc as pfc_r. induction pfc.
+  - intros. assert (exists h1 h2 h3, pfc' = ValidObj ct' h1 h2 h3). apply valid_obj_Valid_Obj.
+    destruct H as [x [y [z id]]]. rewrite id. rewrite Heqpfc_r. apply Hobj.
+  - intros. assert (exists ext' nla' sca' lk' pfd, pfc' = ValidParent ct' c d pfd ext' nla' sca' lk').
+    { apply rel_par_same with ct pfc_r pfc e n o e0.
+      - trivial.
+      - trivial. }
+    destruct H as [ext' [nla' [sca' [lk' [pfd' H']]]]].
+    rewrite H'. rewrite Heqpfc_r. apply Hind. apply IHpfc. trivial.
+Qed.
+
+Lemma pft_left : forall ct, valid_table ct -> (forall c, in_table ct c -> valid_class ct c).
+Proof. intros ct H. admit. Admitted.
+                         
+Lemma val_in_lib_val_in_ct :
+  forall (ct : class_table) (pft : valid_table ct) (c : class) (pfc : valid_class (ct_lib ct) c),
+    valid_class ct c.
+Proof.
+  intros ct pft c pfc.
+  apply pft_left; trivial. apply in_lib_in_table. apply valid_in_lib_in_lib. trivial.
+Qed.
+
+Lemma fields_in_lib_fields_in_ct :
+  forall (ct : class_table) (pft : valid_table ct) (c : class) (pfc_l : valid_class (ct_lib ct) c) (pfc : valid_class ct c),
+    fields (ct_lib ct) c pfc_l = fields ct c pfc.
+Proof.
+  intros ct pft c pfc_l pfc.
+  apply simul_induct_lib with (ct := ct) (c := c) (pfc_l := pfc_l) (pfc := pfc); trivial.
+  intros. simpl. destruct c0; trivial.
+  rewrite H. trivial.
+Qed.
+
+Lemma mtype_in_lib_mtype_in_ct :
+  forall (ct : class_table) (pft : valid_table ct) (c : class) (pfc_l : valid_class (ct_lib ct) c) (pfc : valid_class ct c) mi,
+    mtype (ct_lib ct) mi c pfc_l = mtype ct mi c pfc.
+Proof.
+  intros ct pft c pfc_l pfc mi.
+  apply simul_induct_lib with (ct := ct) (c := c) (pfc_l := pfc_l) (pfc := pfc); trivial.
+  intros. simpl. destruct (lookup_method c0 mi); trivial.
+Qed.
+
+Lemma subtyp_id_lib_sybtyp_id_ct : forall (ct : class_table) (ci : class_id) (di : class_id),
+    valid_table ct -> subtype_id (ct_lib ct) ci di -> subtype_id ct ci di.
+Proof.
+  intros ct ci di pft subtyp_id_lib.
+  induction subtyp_id_lib.
+  - apply SI_Ref. apply in_lib_in_table_id. apply in_ct_lib_in_lib_id. trivial.
+  - apply SI_Sub. apply ext_in_lib_ext_in_ct_id; trivial.
+  - apply SI_Trans with di; trivial.
+Qed.
+
+Lemma typ_in_lib_typ_in_ct :
+  forall (ct : class_table) (pft : valid_table ct) (gamma : context) (e : expr) (ci : class_id),
+    type_of (ct_lib ct) gamma e ci -> type_of ct gamma e ci.
+Proof.
+  intros ct pft gamma e ci typ_in_lib.
+  induction typ_in_lib using type_of_ind_list.
+  - apply T_Var.
+  - apply val_in_lib_val_in_ct in pfc as pfc'; trivial.
+    apply T_Field with c pfc'; trivial.
+    unfold lookup_field. unfold lookup_field in H.
+    assert (fields (ct_lib ct) c pfc = fields ct c pfc'). { apply fields_in_lib_fields_in_ct; trivial. }
+    rewrite <- H0. trivial.
+  - apply val_in_lib_val_in_ct in pfc0 as pfc0'; trivial.
+    apply T_Invk with c0 pfc0' ld ret lc; trivial.
+    * assert (mtype (ct_lib ct) mi c0 pfc0 = mtype ct mi c0 pfc0').
+      { apply mtype_in_lib_mtype_in_ct; trivial. }
+      rewrite <- H6. trivial.
+    * apply Forall_impl with (P := (fun p : class_id * class_id => subtype_id (ct_lib ct) (fst p) (snd p))); trivial.
+      intros a H6. apply subtyp_id_lib_sybtyp_id_ct; trivial.
+  - apply val_in_lib_val_in_ct in pfc as pfc'; trivial.
+    apply T_New with c pfc' lc ld; trivial.
+    + rewrite <- fields_in_lib_fields_in_ct with (pfc_l := pfc); trivial.
+    + apply Forall_impl with (P := (fun p : class_id * class_id => subtype_id (ct_lib ct) (fst p) (snd p))); trivial.
+      intros. apply subtyp_id_lib_sybtyp_id_ct; trivial.
+  - apply T_Cast with di; trivial.
+Qed.
+
+Lemma decl_in_lib_decl_in_ct :
+  forall (ct : class_table) (pft : valid_table ct) (c : class) (pfc : valid_class ct c) (pfc_l : valid_class (ct_lib ct) c) f d,
+    declaring_class (ct_lib ct) c pfc_l f = Some d -> declaring_class ct c pfc f = Some d.
+  intros ct pft c pfc pfc_l.
+  apply simul_induct_lib with (ct := ct) (c := c) (pfc_l := pfc_l) (pfc := pfc); trivial.
+  - clear c pfc pfc_l. intros c d pfd_l pfd ext nla sca lk ext' nla' sca' lk' IHd f e decl_l.
+    simpl in decl_l. simpl. destruct (existsb (fun f' : id => beq_id f' f) (dfields c)); trivial.
+    apply IHd. trivial.
+Qed.
+
+Lemma invk_valid_in_lib_m_in_lib : forall (ct : class_table) e le m (gamma : context),
+    valid_expr (ct_lib ct) gamma (E_Invk e m le) -> exists c, in_lib ct c /\ In m (dmethods c).
+Proof.
+  intros ct e le m gamma val_e.
+  inversion val_e. clear H6. remember pfc as pfc'. induction pfc.
+  - rewrite Heqpfc' in H7. simpl in H7. destruct H7. trivial.
+  - simpl in H7. destruct (existsb (fun m' : id => beq_id m m') (dmethods c)) eqn:exstb. 
+    + exists c. split.
+      * apply in_ct_lib_in_lib. apply valid_in_table. trivial.
+      * rewrite existsb_exists in exstb. destruct exstb as [m' [Inm' Heqm]].
+        rewrite beq_id_true_iff in Heqm. rewrite Heqm. trivial.
+    + apply IHpfc with pfc; trivial.
+      rewrite Heqpfc' in H7. simpl in H7. rewrite exstb in H7. trivial.
+Qed.
 
 Lemma lemma1 : forall (ct : class_table) (c e : class) (m : method_id) (pfc : valid_class ct c),
     mresolve ct m c pfc = Some e -> in_app ct e -> in_app ct c.
@@ -288,76 +750,104 @@ Proof.
       * destruct H. apply H0.
 Qed.
 
-Lemma lemma2 : forall (ct ct' : class_table) (c e e' : class) (m : method_id)
-                 (pfc : valid_class ct c) (pfc' : valid_class ct' c),
-    in_app ct c -> mresolve ct m c pfc = Some e -> mresolve ct' m c pfc' = Some e'  -> ave_rel ct ct' ->
-    in_app ct e \/ in_lib ct' e'.
+Lemma lemma2 : forall ct ct' (pft : ave_rel ct ct') c pfc pfc' e e' m,
+      in_app ct c -> mresolve ct m c pfc = Some e -> mresolve ct' m c pfc' = Some e' ->
+      (in_app ct e \/ in_lib ct' e').
 Proof.
-  intros ct ct' c e e' m pfc pfc' c_in_app c_res_e c_res_e' rel.
-  induction pfc as [| c d pfd IHd c_ext_d not_lib_app app_ext_app].
+  intros ct ct' pft c pfc pfc'. 
+  apply simul_induct with (ct := ct) (ct' := ct') (c := c) (pfc := pfc) (pfc' := pfc'); trivial.
   (* c is Obj *)
-  - unfold mresolve in c_res_e. inversion c_res_e.
+  - contradiction.
   (* c extends d *)
-  - unfold mresolve in c_res_e; fold mresolve in c_res_e.
-    destruct (existsb (fun m' : id => beq_id m m') (dmethods c)) eqn:m_res.
+  - clear c pfc pfc'. intros c d pfd pfd' ext nla sca lk ext' nla' sca' lk' IHd e e' m c_in_app mres_e mres_e'.
+    inversion pft as [ct_val ct'_val keep_app keep_ext keep_lib].
+    simpl in mres_e. destruct (existsb (fun m' : id => beq_id m m') (dmethods c)) eqn:exst.
     (* m-res *)
-    + inversion c_res_e; left; rewrite <- H0; eauto. 
+    + left. inversion mres_e. rewrite <- H0. trivial.
     (* m-res-inh *)
-    + inversion rel as [ct_val ct'_val keep_app keep_ext keep_lib].
-      unfold mresolve in c_res_e'.
-      (* can't induct on pfc and pfc' simultaneously,
-         so manually destruct pfc' and show that it's the same parent *)
-      destruct pfc' as [| c0 d0 pfd' c_ext_d'] eqn:pfc''.
-      * inversion c_res_e'.
-      * fold mresolve in c_res_e'. rewrite m_res in c_res_e'.
-        assert (d = d0) as deq.
-        { apply extends_injective with (ct := ct') (c := c0).
-          -- apply pfc'.
-          -- apply keep_ext.
-             ++ apply c_ext_d.
-             ++ apply in_app_in_table. apply keep_app. apply c_in_app.
-          -- apply c_ext_d'. }
-        destruct app_ext_app as [[d_in_lib _] | [d_in_app _]].
-        (* d in lib - use averroes transformation properties *)
-        -- right. apply mres_lib_in_lib with (m := m) (c := d0) (pfc := pfd').
-           ++ apply keep_lib with (c := c0).
-              ** rewrite <- deq. apply c_ext_d.
-              ** rewrite <- deq. apply d_in_lib.
-              ** apply in_app_in_table. apply keep_app. apply c_in_app.
-           ++ apply c_res_e'.
-        (* d in app - use induction hypothesis *)
-        -- assert (forall pfc' : valid_class ct' d,
-                      in_app ct d ->
-                      mresolve ct' m d pfc' = Some e' -> in_app ct e \/ in_lib ct' e') as IHd'.
-           { intros pfc'0 _ mres'. apply IHd with (pfc' := pfc'0).
-             apply d_in_app. apply c_res_e. apply mres'. }
-           rewrite deq in IHd'.
-           apply IHd' with (pfc' := pfd').
-           ++ rewrite <- deq. apply d_in_app.
-           ++ apply c_res_e'.
+    + simpl in mres_e'. rewrite exst in mres_e'. 
+      destruct sca as [[d_in_lib _] | [d_in_app _]].
+      (* d in lib - use averroes transformation properties *)
+      * right. apply mres_lib_in_lib with m d pfd'; trivial.
+        apply keep_lib with c; trivial. apply in_app_in_table; apply keep_app; trivial.
+      (* d in app - use induction hypothesis *)
+      * apply IHd with m; trivial. 
 Qed.
-
-(* Lemma Forall_imp : forall (A : type) (l : list A)  *)
 
 Lemma lemma3 : forall (ct ct' : class_table) (pft : ave_rel ct ct')
                  (sig sig' : subst) (gamma : context) (e0 : expr),
-    (forall v, alpha ct ct' pft (sig v, sig' v)) -> type_checks ct' gamma e0 ->
-    alpha ct ct' pft (do_sub sig e0, do_sub sig' e0).
+    (forall v, alpha ct ct' pft gamma (EL_Expr (sig v), EL_Expr (sig' v))) -> type_checks ct' gamma e0 ->
+    alpha ct ct' pft gamma (EL_Expr (do_sub sig e0), EL_Expr (do_sub sig' e0)).
 Proof.
   intros ct ct' pft sig sig' gamma e0 rel typ_chk. induction e0 using expr_ind_list.
+  (* Case Var *)
   - eauto.
+  (* Case Field *)
   - simpl; apply Rel_Field. inversion typ_chk; eauto. 
+  (* Case Invk *)
   - simpl; apply Rel_Invk.
     + inversion typ_chk; eauto. 
     + rewrite map_length, map_length; reflexivity.
     + inversion typ_chk. clear H2; clear H3; clear typ_chk; induction l.
       * apply Forall_nil. 
       * inversion H; inversion H6. apply Forall_cons; eauto; eauto.
+  (* Case New *)
   - simpl. inversion typ_chk. apply Rel_New.
     + eauto.
     + rewrite map_length, map_length; reflexivity.
     + clear typ_chk; clear H1; induction l.
       * apply Forall_nil.
       * inversion H; inversion H3. apply Forall_cons; eauto; eauto.
+  (* Case Cast *)
   - apply Rel_Cast; inversion typ_chk; eauto.
+Qed.
+
+Lemma lemma4 : forall (ct ct' : class_table) (pft : ave_rel ct ct')
+                 (sig : subst) (gamma : context) (e0 : expr),
+    (forall v, alpha ct ct' pft gamma (EL_Expr (sig v), EL_Lib)) -> valid_expr (ct_lib ct) gamma e0 ->
+    alpha ct ct' pft gamma (EL_Expr (do_sub sig e0), EL_Lib).
+Proof.
+  intros ct ct' pft sig gamma e0 rel val_e_lib. induction e0 using expr_ind_list.
+  (* Case Var *)
+  - eauto.
+  (* Case Field *)
+  - simpl. inversion val_e_lib as [|x y di0 d0 pfd0 typ_chk_ef0 e_typ_d0 di_d0 f_def val_e0_lib | | |];
+    clear x y H H0.
+    inversion typ_chk_ef0 as [| x y di e_typ_d z typ_chk_e0 | | | ]; clear x y z H H0.
+    remember (declaring_class (ct_lib ct) d0 pfd0 f0) as f_decl in f_def. destruct f_decl. 
+    + inversion pft. assert (valid_class ct d0) as pfd0'.
+      { apply val_in_lib_val_in_ct. trivial. trivial. }
+      apply Rel_Lib_Field with (ci := c) (c := d0) (pfc := pfd0').
+      * apply IHe0. inversion val_e_lib. trivial.
+      * apply decl_in_lib_decl_in_ct with pfd0; trivial. eauto.
+      * apply decl_in_lib_in_lib with d0 pfd0 f0. eauto.
+      * apply typ_in_lib_typ_in_ct. trivial. apply sub_keep_typ. rewrite di_d0. trivial.
+    + destruct f_def. reflexivity.
+  (* Case Invk *)
+  - simpl. inversion val_e_lib.
+    apply Rel_Lib_Invk.
+    + apply invk_valid_in_lib_m_in_lib with e0 l gamma. trivial.
+    + apply IHe0. trivial.
+    (* clean up using Forall principles? *) 
+    + clear H3 H2 val_e_lib. induction l.
+      * simpl. apply Forall_nil.
+      * simpl. apply Forall_cons.
+        -- inversion H. apply H9. inversion H5. trivial.
+        -- apply IHl.
+           ++ inversion H. trivial.
+           ++ inversion H5. trivial.
+  (* Case New *)
+  - simpl. inversion val_e_lib.
+    apply Rel_Lib_New.
+    + apply in_ct_lib_in_lib_id. inversion H2. trivial.
+    + clear H2 H1 val_e_lib. induction l.
+      * simpl. apply Forall_nil.
+      * simpl. apply Forall_cons.
+        -- inversion H. apply H4. inversion H3. trivial. 
+        -- apply IHl.
+           ++ inversion H. trivial.
+           ++ inversion H3. trivial.
+  (* Case Cast *)
+  - simpl. inversion val_e_lib.
+    apply Rel_Lib_Cast. apply IHe0. apply H2.
 Qed.
